Weidenbach_Book/IsaSAT/IsaSAT_Restart_Defs.thy
@@ -260,17 +260,42 @@ definition arena_header_size :: \<open>arena \<Rightarrow> nat \<Rightarrow> nat
   \<open>arena_header_size arena C =
   (if arena_length arena C > 4 then MAX_HEADER_SIZE else MIN_HEADER_SIZE)\<close>
 
-definition update_restart_phases :: \<open>isasat \<Rightarrow> isasat nres\<close> where
-  \<open>update_restart_phases = (\<lambda>S. do {
-     let heur = get_heur S;
+definition update_restart_mode :: \<open>isasat \<Rightarrow> isasat nres\<close> where
+  \<open>update_restart_mode = (\<lambda>S. do {
+    let heur = get_heur S;
+     let stats = get_stats_heur S;
      let lcount = get_global_conflict_count S;
      let vm = get_vmtf_heur S;
      let vm = switch_bump_heur vm;
-     heur \<leftarrow> RETURN (incr_restart_phase heur);
-     heur \<leftarrow> RETURN (if current_restart_phase heur = STABLE_MODE then incr_restart_phase_and_length_end lcount heur else incr_restart_phase_end lcount heur);
-     heur \<leftarrow> RETURN (if current_restart_phase heur = STABLE_MODE then heuristic_reluctant_enable heur else heuristic_reluctant_disable heur);
-     heur \<leftarrow> RETURN (swap_emas heur);
-     RETURN (set_heur_wl_heur heur (set_vmtf_wl_heur vm S))
+     let init_ticks = init_phase_ticks heur;
+     end_of_restart_phase \<leftarrow> RETURN (end_of_restart_phase_st S);
+     let curr = current_restart_phase heur;
+     if init_ticks = 0 \<comment>\<open>This is still the very first phase, here the limit is given by conflicts\<close>
+     then do{
+       if (end_of_restart_phase < lcount) then RETURN (set_heur_wl_heur heur (set_vmtf_wl_heur vm S))
+       else do {
+          let stats = get_stats_heur S;
+          let ticks = stats_ticks_focused stats;
+          heur \<leftarrow> RETURN (if curr \<noteq> STABLE_MODE then heuristic_reluctant_enable heur else heuristic_reluctant_disable heur);
+          heur \<leftarrow> RETURN (incr_restart_phase heur);
+          heur \<leftarrow> RETURN (set_init_phase_ticks ticks heur);
+          heur \<leftarrow> RETURN (swap_emas heur);
+          RETURN (set_heur_wl_heur heur (set_vmtf_wl_heur vm S))
+       }
+     } else do { \<comment>\<open>This is still the very first phase, here the limit is given by ticks\<close>
+        let search_ticks = (if current_restart_phase heur = STABLE_MODE then stats_ticks_stable stats else stats_ticks_focused stats);
+        if (end_of_restart_phase < search_ticks) then RETURN (set_heur_wl_heur heur (set_vmtf_wl_heur vm S))
+        else do {
+          heur \<leftarrow> RETURN (incr_restart_phase heur);
+          heur \<leftarrow> RETURN (if curr \<noteq> STABLE_MODE then heuristic_reluctant_enable heur else heuristic_reluctant_disable heur);
+          let search_ticks = (if curr = STABLE_MODE then stats_ticks_stable stats else stats_ticks_focused stats);
+          let delta = init_ticks * nbstable_phase heur * nbstable_phase heur;
+          let lim = search_ticks + delta;
+          heur \<leftarrow> RETURN (if curr = STABLE_MODE then incr_restart_phase_and_length_end lim heur else incr_restart_phase_end lim heur);
+          heur \<leftarrow> RETURN (swap_emas heur);
+          RETURN (set_heur_wl_heur heur (set_vmtf_wl_heur vm S))
+      }
+    }
   })\<close>
 
 
